lean: hello

lean/hello/Hello.lean
@@ -1,3 +1,32 @@
 -- This module serves as the root of the `Hello` library.
 -- Import modules here that should be built as part of the library.
 import Hello.Basic
+
+#eval 1 + 2
+#eval 1 + 2 * 5
+
+#eval String.removeLeadingSpaces "   a"
+
+#eval if true then 5 else 1
+
+#eval (1 + 2 : Nat)
+#eval (1 + 1.1 : Float)
+#eval (0: Nat)
+#eval (-1: Int)
+
+#check Function.uncurry String.append
+
+def add1 (n: Nat) : Nat := n + 1
+def add  (n: Nat) (k: Nat) : Nat := n + k
+def uncurried_add := Function.uncurry add
+
+theorem add_comm (n m: Nat) : n + m = m + n := by
+  induction n with
+  | zero =>
+    simp
+  | succ n ih =>
+
+
+theorem pointwise_to_add (x y: Nat) : add x y = add y x := by
+  simp [add]
+  apply add_comm
